<?xml version="1.0" encoding="UTF-8"?>

<section xml:id="sec-normal-dist-1" xmlns:xi="http://www.w3.org/2001/XInclude">
  <title>The Normal Distribution II</title>
  <case>
    <title>Assumptions So Far</title>
    <ol>
      <li>
        <p>
          <em>Distribution is radially symmetric.</em>
        </p>
      </li>
      <li>
        <p>
          <em>Probability of landing in a small region is proportional to the size of that region.</em>
        </p>
      </li>
      <li>
        <p>
          <em>Probability of landing in a region monotonically decreases as the distance away from the origin increases.</em>
        </p>
      </li>
    </ol>
    
  </case>
    <p>
      From <xref ref="ex-norm-1"/>, we have that
      <me>g(x) = e^{Ax^2}</me>
      where A is some constant. To ensure <m>g</m> is monotone decreasing, set
      <me>g(x) = e^{-h^2x^2}.</me>

    </p>
    <p>
      We now have a candidate <term>probability density function (PDF)</term> for the <m>x</m> coordinate
      <me>f(x) = \psi e^{-h^2x^2}.</me>
      That is, the probability of the <m>x</m> coordinate of the dart lying in an interval <m>[a,b]</m> is given by
      <me>\int_a^b f(x)dx.</me>
      All that remains of our derivation is specifying the variables <m>\psi</m> and <m>h</m>. This is done by setting
      <me>1 = \int_{-\infty}^\infty f(x) dx = \int_{-\infty}^\infty \psi e^{-h^2x^2} dx</me>
      substituting <m>u = hx</m>, the problem becomes
      <men xml:id="eqn-gauss-posed">\int_{-\infty}^\infty e^{-u^2} dx = \frac{h}{\psi}.</men>
      This is where we come across the <term>Gaussian Integral</term>, an intergral imposibble to compute using standard techniques.
      Luckily for us, multivariable calculus provides all the tools we require. 

    </p>
<subsection xml:id="subsec-gauss">
  <title>The Gaussian Integral</title>
  <p>
    Set <m>I = \int_{-\infty}^\infty e^{-x^2} dx </m>. Then
    <me>I^2 = \int_{-\infty}^\infty e^{-x^2} dx\cdot\int_{-\infty}^\infty e^{-y^2} dy.</me>
    Since the integral <m>\int_{-\infty}^\infty e^{-x^2} dx</m> is constant, we have
    <me>I^2 = \int_{-\infty}^\infty \int_{-\infty}^\infty e^{-x^2} dx\cdot e^{-y^2} dy.</me>
    Since <m>e^{-y^2}</m> is constant with respect to <m>x</m>, we have
    <me>I^2 = \int_{-\infty}^\infty \int_{-\infty}^\infty e^{-x^2}\cdot e^{-y^2} dxdy.</me>
    Simplifying the integrand leaves us with
    <me>I^2 = \int_{-\infty}^\infty \int_{-\infty}^\infty e^{-(x^2+y^2)} dxdy.</me>
    Now we want to make a <term>change of variables</term> into polar coordinates.
    <men xml:id="eqn-polar">\begin{cases}x  = r\text{ cos}(\theta) \\ 
      y = r\text{ sin}(\theta)\end{cases}</men>

    To do this, we must apply a scaling to the integrand (much as we would do for one-dimensional integration). 
    For integration in higher dimensions, this manifests as the <term>Jacobian</term>.
    <me>
      \frac{\partial(x, y)}{\partial(r, \theta)}  = \left|
      \begin{matrix}
      \dfrac{\strut\partial x}{\strut\partial r} \amp \dfrac{\strut\partial x}{\strut\partial \theta}  \\
      \dfrac{\strut\partial y}{\strut\partial r} \amp \dfrac{\strut\partial y}{\strut\partial \theta}
      \end{matrix}
      \right| 
      </me>
      substituting in <xref ref="eqn-polar"/>, we have
      <me>
      \left|
      \begin{matrix}
      \cos(\theta) \amp -r\sin(\theta)  \\
      \sin(\theta) \amp r\cos(\theta)
      \end{matrix}
      \right|  \\
       = r\cos^2(\theta) + r\sin^2(\theta)  \\
       = r.
    </me>
    By choosing appropriate bounds, we now complete the change of variables
    <md>
      <mrow>I^2 =\amp \int_{0}^{2\pi} \int_{0}^\infty e^{-(r^2)} \cdot r \cdot drd\theta</mrow>
      <mrow> =\amp 2\pi \int_{0}^\infty re^{-(r^2)} dr</mrow>
      <mrow> =\amp 2\pi \bigg[-\frac{1}{2}e^{-r^2}\bigg]_0^\infty</mrow>
      <mrow> =\amp 2\pi \bigg(0 + \frac{1}{2}\bigg) = \pi.</mrow>
    </md>
    This leaves us with the satisfying result
    <men xml:id="eqn-gauss-solved"> I = \int_{-\infty}^\infty e^{-x^2} dx = \sqrt{\pi}.</men>
  </p>

</subsection>
</section>